coq/IRR/Simplifications/SimplifyTargeted.v
@@ -1,12 +1,12 @@
 Require Import Koika.KoikaForm.Untyped.UntypedSemantics.
-Require Import Koika.SimpleForm.Interpretation.
-Require Import Koika.SimpleForm.Direction.
-Require Import Koika.SimpleForm.Operations.
-Require Import Koika.SimpleForm.Simplifications.Simplify.
+Require Import Koika.IRR.Interpretation.
+Require Import Koika.IRR.Direction.
+Require Import Koika.IRR.Operations.
+Require Import Koika.IRR.Simplifications.Simplify.
 Require Import Koika.BitsToLists.
 Require Import Koika.KoikaForm.SimpleVal.
 Require Import Koika.KoikaForm.Types.
-Require Import Koika.SimpleForm.SimpleForm.
+Require Import Koika.IRR.IRR.
 Require Import Koika.Utils.EqDec.
 Require Import Koika.Utils.Maps.
 Require Import Koika.Utils.Environments.
@@ -806,7 +806,7 @@ Section SimplifyTargeted.
   Qed.
 
   Definition simplify_sf_targeted
-    (sf: simple_form (rule_name_t := rule_name_t)) (exemptions: PTree.t (list position))
+    (sf: IRR (rule_name_t := rule_name_t)) (exemptions: PTree.t (list position))
   :=
     sf <|
       vars :=
